various refactoring - remove lemma: helping_prophecy_refines - add advanced lemmas: prophecy_refines & helping_refines (cf. prophecy_main & helping_main) - add defs: CFilter.msk_filter_in - add tactics: cfilter_solver, real_mod_solver, mod_eq_solver

apc/APCHeader.v
@@ -5,4 +5,7 @@ From Ordinal Require Export Ordinal Arithmetic Inaccessible.
 
 Module APCHdr.  
   Definition apc := "APC.apc".
+
+  Definition exports : gset string :=
+    {[ apc ]}.
 End APCHdr.
