prophecy/ProphecyFacts.v
@@ -1,44 +1,81 @@
-From CRIS Require Export CRIS CallFilter ProphecyIAproof HelpingFacts HelpingTactics.
-From CRIS Require Export SchI MemI MemA MemIAproof.
+From CRIS Require Export CRIS CallFilter ProphecyIAproof.
 From stdpp Require Import base list.
-
-Lemma CFilter_real_mod `{Σ : GRA} (md : Mod.t) (msk : gset string) :
-  real_mod md → real_mod (CFilter.filter msk md).
-Proof.
-  rewrite /real_mod !map_Forall_lookup /CFilter.filter {2}/Mod.fnsems.
-  intros Hix i x; rewrite lookup_fmap; specialize (Hix i); destruct lookup as [[[? ?]|]|];
-    i; clarify; destruct x; ss; clarify.
-  { rewrite /CFilter.msk_filter /=; eapply (Hix (Some (e, f))); ss. }
-Qed.
 
 Section prophecy.
   Context `{!crisG Γ Σ α β τ Hinv Hsub, !prophGS}.
 
-  (* Lemmas about names *)
-  Local Definition maxlen (s : list string) : nat :=
-    list_max (String.length <$> s).
+  Lemma prophecy_exports_long mn fn
+    (INfn: fn ∈ Prophecy.exports mn)
+    :
+    String.length fn > String.length mn.
+  Proof.
+    revert INfn. rewrite !elem_of_union !elem_of_singleton.
+    rewrite /Prophecy.new /Prophecy.resolve /Prophecy.close.
+    i; des; subst; s; rewrite string_length_app; nia.
+  Qed.
 
-  Local Fixpoint mname_long (n : nat) : string :=
-    match n with
-    | 0 => ""
-    | S n' => "h" +:+ mname_long n'
-    end.
+  Lemma prophecy_refines sz (mds mdt ctx : Mod.t) (mdm : string → Mod.t) (Pm Ps : iProp Σ)
+    (REF1: ∀ Q,
+      refines
+        (mdm (mname_long sz) ★ ProphecyI.t (mname_long sz) ★ CFilter.filter (Prophecy.exports (mname_long sz)) ctx, (Pm ∗ Q)%I)
+        (CFilter.filter (Prophecy.exports (mname_long sz)) mdt ★ ProphecyI.t (mname_long sz) ★ CFilter.filter (Prophecy.exports (mname_long sz)) ctx, Q))
+    (REF2: ∀ Q,
+      refines
+        (mds ★ CFilter.filter (Prophecy.exports (mname_long sz)) ctx, (Ps ∗ Q)%I)
+        (mdm (mname_long sz) ★ ProphecyA.t (mname_long sz) ∅ ★ CFilter.filter (Prophecy.exports (mname_long sz)) ctx, Q))
+    (SZ: sz > max (maxlen (elements (get_fids (dom (Mod.fnsems (mds ★ mdt ★ ctx))))))
+                  (maxlen (Mod.scopes (mds ★ mdt ★ ctx))))
+    (Realmdm: real_mod (mdm (mname_long sz)))
+    (Realctx: real_mod ctx)
+    :
+    refines (mds ★ ctx, Pm ∗ ProphecyA.initial_cond ∗ Ps)%I
+            (mdt ★ ctx, emp%I).
+  Proof.
+    etrans; cycle 1.
+    { eapply ctxr_refines, (CFilter.intro_filter (Prophecy.exports (mname_long sz))). }
 
-  Local Lemma mname_long_length n : String.length (mname_long n) = n.
-  Proof. induction n; ss. rewrite IHn. et. Qed.
+    etrans; cycle 1.
+    { eapply CFilter.intro_module with (mc := ProphecyI.t (mname_long sz)).
+      { econs; [mod_tac|prove_nodup]. }
+      { set_solver. }
+      { intros i Hi1 Hi2; rewrite -elem_of_elements in Hi1; eapply elem_of_maxlen in Hi1.
+        eapply prophecy_exports_long in Hi2. rewrite mname_long_length in Hi2.
+        rewrite Mod.dom_fnsems_add maxlen_get_fids_union in SZ. nia.
+      }
+      { set_solver+. }
+      { set_solver+. }
+    }
+    rewrite CFilter.filter_app.
+    etrans; cycle 1.
+    { rewrite -assoc (comm _ _ (ProphecyI.t _)). apply REF1. }
+    etrans; cycle 1.
+    { rewrite (comm _ (ProphecyI.t _)) assoc.
+      eapply ProphIA.adequacy_refines; eauto.
+      eapply real_mod_add; eauto using CFilter.real_mod.
+    }
+    etrans; cycle 1.
+    { rewrite -assoc (comm _ _ (ProphecyA.t _ _)). apply REF2. }
+    etrans; cycle 1.
+    { eapply ctxr_refines. ctxr_rotate. ctxr_drop.
+      eapply CFilter.intro_filter. }
+    erewrite <-!CFilter.filter_app. ctxr_norm.
+    etrans; cycle 1.
+    { eapply CFilter.elim_filter.
+      intros i Hi1 Hi2; rewrite -elem_of_elements in Hi1; eapply elem_of_maxlen in Hi1.
+      rewrite Mod.dom_fnsems_add maxlen_get_fids_union in Hi1.
+      eapply prophecy_exports_long in Hi2. rewrite mname_long_length in Hi2.
+      do 2 rewrite Mod.dom_fnsems_add maxlen_get_fids_union in SZ. nia.
+    }
 
-  Local Lemma elem_of_maxlen (fn : string) (s : list string) :
-    fn ∈ s → String.length fn ≤ maxlen s.
-  Proof. i; eapply max_list_elem_of_le, elem_of_list_fmap; esplits; eauto. Qed.
+    rewrite comm.
+    eapply ctxr_refines, ctxr_cond_strengthen; iIntros "[$ [$ $]]".
+  Qed.
 
-  Local Lemma maxlen_union s1 s2 : maxlen (s1 ++ s2) = maxlen s1 `max` maxlen s2.
-  Proof. rewrite /maxlen fmap_app list_max_app //. Qed.
-
-  Lemma prophecy_refines (mds mdt ctx : Mod.t) (mdm : string → Mod.t) (Pm Ps : iProp Σ) :
+  Lemma prophecy_main (mds mdt ctx : Mod.t) (mdm : string → Mod.t) (Pm Ps : iProp Σ) :
     (∀ mn,
       ctx_refines
         (mdm mn ★ ProphecyI.t mn, Pm)
-        (CFilter.filter (ProphecyName.exports mn) mdt ★ ProphecyI.t mn, emp%I)) →
+        (CFilter.filter (Prophecy.exports mn) mdt ★ ProphecyI.t mn, emp%I)) →
     (∀ mn,
       ctx_refines
         (mds, Ps)
@@ -47,172 +84,15 @@ Section prophecy.
     real_mod ctx →
     refines (mds ★ ctx, Pm ∗ ProphecyA.initial_cond ∗ Ps)%I (mdt ★ ctx, emp%I).
   Proof.
-    intros Hproph Hreal ? ?.
-    set (mn := maxlen
-      (elements (set_omap (λ a, match a with | fid fn => Some fn | _ => None end) (dom (Mod.fnsems (mdt ★ ctx))) : gset string) ++
-       elements (set_omap (λ a, match a with | fid fn => Some fn | _ => None end) (dom (Mod.fnsems (ctx ★ mds))) : gset string) ++
-      Mod.scopes mdt ++ Mod.scopes ctx ++ Mod.scopes mds)).
-    etrans; cycle 1.
-    { eapply ctxr_refines,
-        CFilter.intro_filter with (fns := ProphecyName.exports (mname_long (S mn))). }
-    etrans; cycle 1.
-    { eapply CFilter.intro_module with (mc := ProphecyI.t (mname_long (S mn))).
-      { econs; [mod_tac|prove_nodup]. }
-      { set_solver. }
-      { intros i Hi1 Hi2; rewrite -elem_of_elements in Hi1; eapply elem_of_maxlen in Hi1;
-        set_unfold; des; subst mn; subst; ss;
-          rewrite ?mname_long_length ?maxlen_union in Hi1; lia.
-      }
-      { set_solver+. }
-      { set_solver+. }
-    }
-    rewrite CFilter.filter_app.
-    etrans; cycle 1.
-    { eapply ctxr_refines.
-      ctxr_rotate. ctxr_drop. ctxr_rotate.
-      eapply (Hproph (mname_long (S mn))).
-    }
-    etrans; cycle 1.
-    { rewrite comm -assoc (Mod.add_comm (ProphecyI.t _)) assoc.
-      eapply ProphIA.adequacy_refines; eauto.
-      eapply real_mod_add; eauto using CFilter_real_mod.
-    }
-    etrans; cycle 1.
-    { eapply ctxr_refines. ctxr_rotate. ctxr_drop. ctxr_rotate. eapply Hreal. }
-    etrans; cycle 1.
-    { eapply ctxr_refines. ctxr_drop. eapply CFilter.intro_filter. }
-    erewrite <-!CFilter.filter_app. ctxr_norm.
-    etrans; cycle 1.
-    { eapply CFilter.elim_filter.
-      intros i Hi1 Hi2; rewrite -elem_of_elements in Hi1; eapply elem_of_maxlen in Hi1;
-        set_unfold; des; subst mn; subst; ss;
-          rewrite ?mname_long_length ?maxlen_union in Hi1; lia.
-    }
-
-    rewrite Mod.add_comm.
-    eapply ctxr_refines, ctxr_cond_strengthen; iIntros "[$ [$ $]]".
+    intros REF1 REF2 Rmdm Rctx; s.
+    set (sz := S (max
+                 (maxlen (elements (get_fids (dom (Mod.fnsems (mds ★ mdt ★ ctx))))))
+                 (maxlen (Mod.scopes (mds ★ mdt ★ ctx))))).
+    eapply prophecy_refines with (sz:=sz); i; eauto using prophecy_exports_long; try nia.
+    - eapply ctxr_refines. rewrite !assoc -{2}(left_id _ bi_sep Q).
+      eapply ctxr_frameR, ctxr_cond_frameR. eapply REF1.
+    - eapply ctxr_refines. rewrite !assoc -{2}(left_id _ bi_sep Q).
+      eapply ctxr_frameR, ctxr_cond_frameR. eapply REF2.
   Qed.
 
-  Lemma helping_prophecy_refines
-      `{!memGS, !inG (helpingR jobID retID) Γ}
-      (mds mdt ctx : Mod.t) (mdp mdm : string → Mod.t) csl genv sp_mem sp_help
-      (jobs : jobID → itree crisE retID) :
-    let fns mn := ProphecyName.exports mn ∪ Helping.exports mn in
-    (∀ mn,
-      ctx_refines
-        (mdp mn ★ ProphecyI.t mn, emp%I) (CFilter.filter (fns mn) mdt ★ ProphecyI.t mn, emp%I)) →
-    (∀ mn,
-      ctx_refines
-        (mdm mn ★ HelpingOn.t mn jobs sp_help ★ MemA.t sp_mem ★ ProphecyA.t mn ∅, 
-          helping_auth 1 ∅ ∗ free_id top1)%I
-        (mdp mn ★ HelpingDummy.t mn ★ MemA.t sp_mem ★ ProphecyA.t mn ∅, emp)%I) →
-    (∀ mn, ctx_refines (mds, emp%I) (mdm mn ★ HelpingOff.t mn jobs sp_help, emp)%I) →
-    real_mod ctx →
-    (∀ mn, real_mod (mdp mn)) →
-    refines
-      (mds ★ MemA.t sp_mem ★ SchI.t ★ ctx,
-        MemA.init_cond csl genv ∗ ProphecyA.initial_cond ∗ helping_auth 1 ∅ ∗ free_id top1%type)%I
-      (mdt ★ MemI.t csl genv ★ SchI.t ★ ctx,
-        emp%I).
-  Proof.
-    intros fns Hproph_insert Hmain Herase Hctx_real Hmdp_real.
-    assert (Hadd_wf : ∀ mn, Mod.wf (ProphecyI.t mn ★ HelpingDummy.t mn)).
-    { i; econs; [mod_tac|prove_nodup]. }
-    set (l := maxlen
-      (elements (set_omap (λ a, match a with | fid fn => Some fn | _ => None end) (dom (Mod.fnsems (SchI.t ★ ctx ★ MemA.t sp_mem ★ mds))) : gset string) ++
-       elements (set_omap (λ a, match a with | fid fn => Some fn | _ => None end) (dom (Mod.fnsems (mdt ★ MemI.t csl genv ★ SchI.t ★ ctx))) : gset string) ++
-       Mod.scopes (mdt ★ MemI.t csl genv ★ SchI.t ★ ctx) ++
-      Mod.scopes mdt ++ Mod.scopes ctx ++ Mod.scopes mds)).
-    set (mn := mname_long (S l)).
-    assert (mn ∉ Mod.scopes (mdt ★ MemI.t csl genv ★ SchI.t ★ ctx)) as Hmn.
-    { intros Hcontra%elem_of_maxlen; subst mn l.
-      rewrite !mname_long_length ?maxlen_union in Hcontra; lia.
-    }
-    etrans; cycle 1.
-    { eapply ctxr_refines, CFilter.intro_filter with (fns := fns mn). }
-    etrans; cycle 1.
-    { eapply CFilter.intro_module with (mc := ProphecyI.t mn ★ HelpingDummy.t mn).
-      { apply Hadd_wf. }
-      { revert Hmn; generalize mn; clear dependent mn. intros ? ?. set_solver+Hmn. }
-      { intros i Hi1 Hi2; rewrite -elem_of_elements in Hi1; eapply elem_of_maxlen in Hi1.
-        subst fns; set_unfold in Hi2; des; subst mn l; subst;
-          rewrite string_length_app ?mname_long_length ?maxlen_union in Hi1; lia.
-      }
-      { clear. generalize mn; clear dependent mn l; subst fns; intros ?.
-        rewrite Mod.dom_fnsems_add set_omap_union; set_solver. }
-      { clear. generalize mn; clear dependent mn l; intros ?.
-        rewrite Mod.dom_fnsems_add. set_solver+. }
-    }
-    do 2 rewrite CFilter.filter_app.
-    etrans; cycle 1.
-    { eapply ctxr_refines.
-      ctxr_rotate. do 2 ctxr_drop. ctxr_rotate. ctxr_drop.
-      eapply (Hproph_insert).
-    }
-    etrans; cycle 1.
-    { rewrite ?assoc.
-      eapply ProphIA.adequacy_refines; eauto.
-      rewrite -!assoc CFilter.filter_app.
-      repeat eapply real_mod_add; eauto using CFilter_real_mod.
-      { apply CFilter_real_mod. rewrite /real_mod.
-        clear dependent mn l.
-        let real_tac :=
-          (split; ss; intros ??; destruct excluded_middle_informative; ss) in
-        mod_tac real_tac.
-       }
-      { apply CFilter_real_mod. rewrite /real_mod.
-        clear.
-        let real_tac :=
-          (split; ss; intros ??; destruct excluded_middle_informative; ss) in
-        mod_tac real_tac.
-      }
-      { rewrite /real_mod.
-        clear. generalize mn; clear dependent mn l; intros ?.
-        let real_tac :=
-          (split; ss; intros ??; destruct excluded_middle_informative; ss) in
-        mod_tac real_tac.
-      }
-    }
-    etrans; cycle 1.
-    { eapply ctxr_refines. ctxr_rotate. do 4 ctxr_drop.
-      clear. generalize mn; clear dependent mn l; intros ?.
-      eapply main_adequacy, MemIA.sim; set_solver.
-    }
-    etrans; cycle 1.
-    { eapply ctxr_refines.
-      ctxr_drop. ctxr_swap. do 2 ctxr_rotate. ctxr_swap. do 2 ctxr_rotate.
-      eapply Hmain.
-    }
-    rewrite CFilter.filter_app.
-    etrans; cycle 1.
-    { eapply ctxr_refines. ctxr_rotate. ctxr_drop. ctxr_drop. ctxr_swap. ctxr_drop.
-      ctxr_swap. ctxr_drop.
-      eapply helping_onoff_correct; eauto.
-      clear. generalize mn; clear dependent mn l; intros ?.
-      set_solver.
-    }
-    etrans; cycle 1.
-    { eapply ctxr_refines. ctxr_drop. do 2 (ctxr_swap; ctxr_drop). rewrite /mod_src.
-      do 2 ctxr_rotate. ctxr_drop. eapply Herase.
-    }
-    etrans; cycle 1.
-    { eapply ctxr_refines. do 2 ctxr_drop. ctxr_rotate. do 2 ctxr_drop. eapply elim_module. }
-    etrans; cycle 1.
-    { eapply ctxr_refines. ctxr_rotate. ctxr_drop. ctxr_swap; ctxr_drop. rewrite left_id.
-      erewrite <-!CFilter.filter_app. refl.
-    }
-    etrans; cycle 1.
-    { eapply ctxr_refines. do 2 ctxr_rotate. ctxr_drop. eapply CFilter.intro_filter. }
-    erewrite <-!CFilter.filter_app.
-    etrans; cycle 1.
-    { eapply CFilter.elim_filter.
-      rewrite -assoc.
-      intros i Hi1 Hi2; rewrite -elem_of_elements in Hi1; eapply elem_of_maxlen in Hi1.
-      subst fns; set_unfold in Hi2; des; subst mn l; subst;
-        rewrite string_length_app ?mname_long_length ?maxlen_union in Hi1; lia.
-    }
-    eapply ctxr_refines.
-    ctxr_norm. do 3 ctxr_rotate. ctxr_drop. do 2 ctxr_rotate. ctxr_drop.
-    eapply ctxr_cond_strengthen; iIntros "[$ [$ $]]".
-  Qed.
 End prophecy.
